verification/DisposedBloodList.dfy
@@ -12,6 +12,16 @@ class DisposedBloodList
         && forall i :: 0 <= i < upto ==> list[i] != null
     }
 
+    predicate UniqueId()
+    requires Valid(); ensures Valid();
+    requires list != null 
+    requires 0 <= upto <= list.Length
+    requires forall i :: 0 <= i < upto ==> list[i] != null
+    reads this, this.list, this`upto, set m | 0 <= m < upto :: list[m]`id;
+    {
+        forall j,k:: 0<=j<k<upto ==> list[j].id != list[k].id
+    }
+
     constructor(size: int)
     requires size > 0;
     ensures Valid(); 
@@ -26,7 +36,10 @@ class DisposedBloodList
 
     method addBlood(blood: DisposedBlood)
     ensures Valid(); requires Valid();
+    requires UniqueId(); ensures UniqueId();
     requires blood != null
+    requires forall i :: 0 <= i < upto  ==> list[i]!=null;
+    requires forall i :: 0 <= i < upto  ==> list[i].id != blood.id;
     ensures upto > 0
     ensures list[upto-1] == blood;
     ensures upto == old(upto) + 1;
@@ -47,44 +60,68 @@ class DisposedBloodList
         }
         assert upto < list.Length;
         list[upto], upto := blood, upto + 1;
-
     }
 
-    
-    method extractBlood(id: int) returns (bloodFound: bool, blood: DisposedBlood)
-    ensures Valid(); requires Valid();
+    method getBlood(id: int) returns (blood: DisposedBlood)
+    requires Valid(); ensures Valid();
+    requires UniqueId(); ensures UniqueId();
+    ensures blood != null ==> exists t :: 0 <= t < upto && list[t] == blood;
+    ensures blood == null ==> forall t :: 0 <= t < upto ==> list[t] != blood;
+    ensures blood != null ==> blood.id == id;
+    ensures (exists t :: 0 <= t < old(upto) && old(list[t]).id == id) ==> blood != null;
+    ensures (forall t :: 0 <= t < old(upto) ==> old(list[t]).id != id) ==> blood == null;
+    ensures multiset(old(list[0..old(upto)])) == multiset(list[0..upto]);
+    ensures forall t :: 0 <= t < upto ==> list[t] == old(list[t]);
+    ensures upto == old(upto);
+
+    {
+        var i:= 0;
+        blood := null;
+        while (i < upto) 
+        invariant i <= upto;
+        invariant blood != null ==> exists t :: 0 <= t <= i && list[t] == blood;
+        invariant (exists t :: 0 <= t < old(i) && old(list[t]).id == id) ==> blood != null;
+        invariant (forall t :: 0 <= t < old(i) ==> old(list[t]).id != id) ==> blood == null;
+        {
+            if list[i].id == id {
+                blood := list[i];
+                break;
+            }
+            i := i + 1;
+        }
+    }
+
+    method removeBlood(blood: DisposedBlood)
+    requires Valid(); ensures Valid();
+    requires UniqueId(); ensures UniqueId();
+    modifies this.list, this`upto
     requires upto > 0;
-    ensures !bloodFound  ==> upto == old(upto);
-    ensures !bloodFound ==> old(list[0..upto]) == list[0..upto];
-    ensures bloodFound ==> (exists t :: 0 <= t < old(upto) && old(list[t]) == blood
+    requires exists t :: 0 <= t < upto && list[t] == blood;
+    ensures upto == old(upto) - 1;
+    ensures blood == old(blood);
+    ensures (exists t :: 0 <= t < old(upto) && old(list[t]) == blood
                     && (forall k :: 0 <= k < t ==> list[k] == old(list[k]))
                     && (forall q :: t < q < old(upto) ==> list[q-1] == old(list[q]))
                     );
-    ensures blood != null ==> blood.id == id;
-    ensures (exists t :: 0 <= t < old(upto) && old(list[t]).id == id) ==> bloodFound;
-    ensures (forall t :: 0 <= t < old(upto) ==> old(list[t]).id != id) ==> !bloodFound;
-    ensures bloodFound ==> upto == old(upto) - 1;
-    ensures bloodFound ==> blood.id == id;
-    modifies this.list, this`upto;
+    ensures (forall t :: 0 <= t < upto ==> list[t].id != blood.id);
     {
-        bloodFound := false;
-        blood := null;
         var i:=0;
+        var bloodFound := false;
         var bloodIndex := -1;
-        while i < upto
+        while i <= upto
         invariant 0 <= i <= upto;
         invariant forall k :: 0 <= k < i ==> list[k] != blood;
-        invariant forall j :: 0 <= j < i ==> list[j] == old(list[j])
-        invariant (exists t :: 0 <= t < i && list[t].id == id) ==> bloodFound;
+        invariant forall j :: 0 <= j < i ==> list[j] == old(list[j]);
+        invariant (exists t :: 0 <= t < i && list[t] == blood) ==> bloodFound;
+        invariant bloodFound ==> forall l :: bloodIndex < l < i ==> list[l-1] == old(list[l]);
         invariant forall t :: 0 <= t < old(upto) && old(list[t])!= blood ==> (exists k :: 0 <= k < upto && old(list[t]) == list[k]);
-        invariant bloodFound ==> forall l :: bloodIndex < l < i ==> list[l-1] == old(list[l])
         decreases upto - i;
+
         {
-            if list[i].id == id
+            if list[i] == blood
             {
                 bloodFound := true;
                 bloodIndex := i;
-                blood := list[i];
                 forall(j | i < j < upto)
                 {
                     list[j - 1] := list[j];
@@ -94,15 +131,62 @@ class DisposedBloodList
             }
             i := i + 1;
         }
-
+    }
+    
+    method extractBlood(id: int) returns (blood: DisposedBlood)
+    requires Valid(); ensures Valid();
+    requires UniqueId(); ensures UniqueId();
+    ensures blood != null ==> upto == old(upto-1);
+    ensures blood == null ==> upto == old(upto);
+    ensures blood == null ==> old(list[0..upto]) == list[0..upto];
+    ensures (blood != null) ==> (exists t :: 0 <= t < old(upto) && old(list[t]) == blood
+                            && old(list[0..t]) == list[0..t]
+                            && old(list[t+1..old(upto)]) == list[t..upto]
+                            );
+    ensures (blood != null) ==> (forall t :: 0 <= t < upto ==> list[t].id != id);
+    ensures blood != null ==> blood.id == id;
+    ensures (exists t :: 0 <= t < old(upto) && old(list[t]).id == id) ==> blood != null;
+    ensures (forall t :: 0 <= t < old(upto) ==> old(list[t]).id != id) ==> blood == null;
+    modifies this.list, this`upto
+    {
+        blood := getBlood(id);
+        if(blood != null){
+            removeBlood(blood);
+        }
     }
 }
 
-method Main()
-{
-    var blood := new DisposedBlood(0);
-    var blood2 := new DisposedBlood(1);
-    var blood3 := new DisposedBlood(2);
-    assert blood.id == 0;
-    assert blood2.id == 1;
-}
+// method Main()
+// {
+//     var blood := new DisposedBlood(0);
+//     var blood2 := new DisposedBlood(1);
+//     var blood3 := new DisposedBlood(2);
+//     assert blood.id == 0;
+//     assert blood2.id == 1;
+//     var bloodlist := new DisposedBloodList(2);
+//     bloodlist.addBlood(blood);
+//     assert bloodlist.list[0] == blood;
+//     assert bloodlist.upto == 1;
+//     bloodlist.addBlood(blood2);
+//     assert bloodlist.list[1] == blood2;
+//     assert bloodlist.list[0] == blood;
+//     bloodlist.addBlood(blood3);
+//     assert bloodlist.list[0] == blood;
+//     assert bloodlist.list[1] == blood2;
+//     assert bloodlist.list[2] == blood3;
+//     assert bloodlist.upto == 3;
+
+//     // id = 5 does't exist
+//     var removed := bloodlist.extractBlood(5);
+//     assert removed == null;
+//     assert bloodlist.upto == 3;
+
+//     var removed1 := bloodlist.extractBlood(blood3.id);
+//     assert removed1.id == blood3.id;
+//     assert bloodlist.upto == 2;
+
+//     // id = 5 does't exist
+//     var removed2 := bloodlist.extractBlood(5);
+//     assert removed2 == null;
+//     assert bloodlist.upto == 2;
+// }
